src/Env.v
@@ -650,6 +650,18 @@ Section fin.
             (cc x)
       end.
 
+  Variable a : A.
+  Variable b : B a.
+  Fixpoint hlistIn (ls : list A) : hlist ls -> Prop :=
+    match ls as ls return hlist ls -> Prop with
+      | nil => fun _ => False
+      | hd :: tl => fun hl =>
+        (exists pf : a = hd, hlist_hd hl = match pf in _ = t return B t with
+                                             | refl_equal => b
+                                           end)
+        \/ hlistIn (hlist_tl hl)
+    end.
+
 End fin.
 
 Implicit Arguments FO [A x ls].
